share/pulse/examples/dice/cbor/CDDL.Spec.MapGroupGen.fsti
@@ -108,10 +108,95 @@ val is_sublist_of_prefix
   (ensures (l1 `is_sublist_of` (l1 `List.Tot.append` l2)))
   [SMTPat (l1 `List.Tot.append` l2)]
 
+[@@erasable]
+val ghost_map (key value: Type0) : Type0
+
+val apply_ghost_map (#key #value: Type0) (m: ghost_map key value) (k: key) : GTot (option value)
+
+val ghost_map_ext (#key #value: Type0) (m1 m2: ghost_map key value) : Lemma
+  (requires forall x . apply_ghost_map m1 x == apply_ghost_map m2 x)
+  (ensures m1 == m2)
+
+let ghost_map_mem (#key #value: Type) (kv: (key & value)) (f: ghost_map key value) : Tot prop =
+  apply_ghost_map f (fst kv) == Some (snd kv)
+
+val ghost_map_equiv (#key #value: Type) (f1 f2: ghost_map key value) : Lemma
+  (requires (forall kv . ghost_map_mem kv f1 <==> ghost_map_mem kv f2))
+  (ensures f1 == f2)
+
+let ghost_map_defined (#key #value: Type) (k: key) (f: ghost_map key value) : Tot prop =
+  Some? (apply_ghost_map f k)
+
+let ghost_map_disjoint (#key #value1 #value2: Type) (f1: ghost_map key value1) (f2: ghost_map key value2) : Tot prop =
+  (forall k . ~ (ghost_map_defined k f1 /\ ghost_map_defined k f2))
+
+val ghost_map_empty (#key #value: Type) : Tot (ghost_map key value)
+
+val apply_ghost_map_empty (#key #value: Type) (k: key) : Lemma
+  (apply_ghost_map (ghost_map_empty #key #value) k == None)
+  [SMTPat (apply_ghost_map (ghost_map_empty #key #value) k)]
+
+val ghost_map_singleton (#key #value: Type) (k: key) (v: value) : Tot (ghost_map key value)
+
+val apply_ghost_map_singleton (#key #value: Type) (k: key) (v: value) (k': key) : Lemma
+  (let res = apply_ghost_map (ghost_map_singleton k v) k' in
+    (k == k' ==> res == Some v) /\ ((~ (k == k')) ==> res == None))
+  [SMTPat (apply_ghost_map (ghost_map_singleton k v) k')]
+
+val ghost_map_union (#key #value: Type) (m1 m2: ghost_map key value) : Tot (ghost_map key value)
+
+val apply_ghost_map_union (#key #value: Type) (m1 m2: ghost_map key value) (k: key) : Lemma
+  (apply_ghost_map (ghost_map_union m1 m2) k == begin match apply_ghost_map m1 k with
+    | Some v -> Some v
+    | None -> apply_ghost_map m2 k
+  end)
+  [SMTPat (apply_ghost_map (ghost_map_union m1 m2) k)]
+
+let ghost_map_disjoint_mem_union (#key #value: Type) (m1 m2: ghost_map key value) (xv: (key & value)) : Lemma
+  (requires ghost_map_disjoint m1 m2)
+  (ensures ghost_map_mem xv (m1 `ghost_map_union` m2) <==> ghost_map_mem xv m1 \/ ghost_map_mem xv m2)
+= ()
+
+let ghost_map_disjoint_mem_union' (#key #value: Type) (m1 m2: ghost_map key value) (_: squash (ghost_map_disjoint m1 m2)) : Lemma
+  (ensures forall xv . ghost_map_mem xv (m1 `ghost_map_union` m2) <==> ghost_map_mem xv m1 \/ ghost_map_mem xv m2)
+= ()
+
+val ghost_map_disjoint_union (#key #value: Type) (m1 m2: ghost_map key value) : Lemma
+  (requires ghost_map_disjoint m1 m2)
+  (ensures m1 `ghost_map_union` m2 == m2 `ghost_map_union` m1)
+
+let map_group_item_post
+  (l: list (Cbor.raw_data_item & Cbor.raw_data_item))
+  (l': (ghost_map Cbor.raw_data_item Cbor.raw_data_item & list (Cbor.raw_data_item & Cbor.raw_data_item)))
+: Tot prop
+=
+  (snd l' `is_sublist_of` l) /\
+  (forall x . ~ (ghost_map_defined x (fst l') /\ List.Tot.memP x (List.Tot.map fst (snd l')))) /\
+  (forall x . (ghost_map_mem x (fst l') \/ List.Tot.memP x (snd l')) <==> List.Tot.memP x l)
+
 let cbor_map_pred (l: list (Cbor.raw_data_item & Cbor.raw_data_item)) : Tot prop =
   List.Tot.no_repeats_p (List.Tot.map fst l)
 
 let cbor_map : Type0 = (l: list (Cbor.raw_data_item & Cbor.raw_data_item) { cbor_map_pred l })
+
+val map_group_item_post_prop
+  (l: cbor_map)
+  (l': (ghost_map Cbor.raw_data_item Cbor.raw_data_item & list (Cbor.raw_data_item & Cbor.raw_data_item)))
+: Lemma
+  (requires (map_group_item_post l l'))
+  (ensures (
+    List.Tot.no_repeats_p (List.Tot.map fst (snd l')) /\
+    (forall xy . ~ (ghost_map_mem xy (fst l') /\ List.Tot.memP xy (snd l'))) /\
+    (forall x . Cbor.list_ghost_assoc x l == begin match apply_ghost_map (fst l') x with
+    | Some y -> Some y
+    | None -> Cbor.list_ghost_assoc x (snd l')
+    end) /\
+    (forall x . Cbor.list_ghost_assoc x l == begin match Cbor.list_ghost_assoc x (snd l') with
+    | Some y -> Some y
+    | None -> apply_ghost_map (fst l') x
+    end)
+  ))
+  [SMTPat (map_group_item_post l l')]
 
 val cbor_map_is_sublist_of
   (l1 l2: list (Cbor.raw_data_item & Cbor.raw_data_item))
@@ -164,16 +249,98 @@ let map_group_match_item_for
 : Tot map_group
 = map_group_match_item (t_literal k) ty
 
+val ghost_map_filter
+  (#key #value: Type)
+  (f: (key & value) -> GTot bool)
+  (m: ghost_map key value)
+: ghost_map key value
+
+val apply_ghost_map_filter
+  (#key #value: Type)
+  (f: (key & value) -> GTot bool)
+  (m: ghost_map key value)
+  (k: key)
+: Lemma
+  (apply_ghost_map (ghost_map_filter f m) k == begin match apply_ghost_map m k with
+    | None -> None
+    | Some v -> if f (k, v) then Some v else None
+  end)
+  [SMTPat (apply_ghost_map (ghost_map_filter f m) k)]
+
+let ghost_map_filter_ext
+  (#key #value: Type)
+  (f1 f2: (key & value) -> GTot bool)
+  (m: ghost_map key value)
+: Lemma
+  (requires forall x . f1 x == f2 x)
+  (ensures ghost_map_filter f1 m == ghost_map_filter f2 m)
+= ghost_map_equiv (ghost_map_filter f1 m) (ghost_map_filter f2 m)
+
+val ghost_map_of_list
+  (#key #value: Type)
+  (l: list (key & value))
+: ghost_map key value
+
+val apply_ghost_map_of_list
+  (#key #value: Type)
+  (l: list (key & value))
+  (k: key)
+: Lemma
+  (apply_ghost_map (ghost_map_of_list l) k == Cbor.list_ghost_assoc k l)
+  [SMTPat (apply_ghost_map (ghost_map_of_list l) k)]
+
+val ghost_map_of_list_singleton
+  (#key #value: Type)
+  (kv: (key & value))
+: Lemma
+  (ghost_map_of_list [kv] == ghost_map_singleton (fst kv) (snd kv))
+  [SMTPat (ghost_map_of_list [kv])]
+
+val ghost_map_of_list_append
+  (#key #value: Type)
+  (l1 l2: list (key & value))
+: Lemma
+  (ghost_map_of_list (List.Tot.append l1 l2) == ghost_map_of_list l1 `ghost_map_union` ghost_map_of_list l2)
+
+val ghost_map_of_list_mem_gen
+  (#key #value: Type)
+  (l: list (key & value))
+  (prf: squash (List.Tot.no_repeats_p (List.Tot.map fst l)))
+  (x: (key & value))
+: Lemma
+  (ghost_map_mem x (ghost_map_of_list l) <==> List.Tot.memP x l)
+
+let ghost_map_of_list_mem
+  (l: cbor_map)
+  (x: (Cbor.raw_data_item & Cbor.raw_data_item))
+: Lemma
+  (ghost_map_mem x (ghost_map_of_list l) <==> List.Tot.memP x l)
+= ghost_map_of_list_mem_gen l () x
+
+val ghost_map_filter_of_list
+  (f: _ -> bool)
+  (l: cbor_map)
+: Lemma
+  (ghost_map_filter f (ghost_map_of_list l) == ghost_map_of_list (List.Tot.filter f l))
+
+val map_group_zero_or_more_zero_or_one_eq
+  (m: map_group)
+: Lemma
+  (map_group_zero_or_more (map_group_zero_or_one m) == map_group_zero_or_more m)
+
 [@@erasable]
 noeq
 type map_group_result =
 | MapGroupFail
-| MapGroupDet of cbor_map
+| MapGroupDet:
+  (consumed: ghost_map Cbor.raw_data_item Cbor.raw_data_item) ->
+  (remaining: cbor_map) ->
+  map_group_result
 | MapGroupNonDet
 
 let map_group_result_prop (l: cbor_map) (r: map_group_result) : Tot prop =
   match r with
-  | MapGroupDet m -> m `is_sublist_of` l
+  | MapGroupDet c m -> map_group_item_post l (c, m)
   | _ -> True
 
 val apply_map_group_det (m: map_group) (l: cbor_map) : Pure map_group_result
@@ -184,13 +351,13 @@ val apply_map_group_det_always_false (l: cbor_map) : Lemma
   (apply_map_group_det map_group_always_false l == MapGroupFail)
   [SMTPat (apply_map_group_det map_group_always_false l)]
 
-val apply_map_group_det_end (l: cbor_map) : Lemma
-  (apply_map_group_det map_group_end l == (if Nil? l then MapGroupDet l else MapGroupFail))
-  [SMTPat (apply_map_group_det map_group_end l)]
-
 val apply_map_group_det_nop (l: cbor_map) : Lemma
-  (apply_map_group_det map_group_nop l == MapGroupDet l)
+  (apply_map_group_det map_group_nop l == MapGroupDet ghost_map_empty l)
   [SMTPat (apply_map_group_det map_group_nop l)]
+
+val apply_map_group_det_end (l: cbor_map) : Lemma
+  (apply_map_group_det map_group_end l == (if Nil? l then MapGroupDet ghost_map_empty l else MapGroupFail))
+  [SMTPat (apply_map_group_det map_group_end l)]
 
 val apply_map_group_det_map_group_equiv (m1 m2: map_group) : Lemma
   (requires
@@ -215,7 +382,7 @@ let apply_map_group_det_map_group_equiv0 (m1 m2: map_group)
 val apply_map_group_det_choice (m1 m2: map_group) (l: cbor_map) : Lemma
   (match apply_map_group_det m1 l with
   | MapGroupFail -> apply_map_group_det (m1 `map_group_choice` m2) l == apply_map_group_det m2 l
-  | MapGroupDet l1 -> apply_map_group_det (m1 `map_group_choice` m2) l == MapGroupDet l1
+  | MapGroupDet c1 l1 -> apply_map_group_det (m1 `map_group_choice` m2) l == MapGroupDet c1 l1
   | _ -> True
   )
   [SMTPat (apply_map_group_det (map_group_choice m1 m2) l)]
@@ -223,14 +390,18 @@ val apply_map_group_det_choice (m1 m2: map_group) (l: cbor_map) : Lemma
 val apply_map_group_det_concat (m1 m2: map_group) (l: cbor_map) : Lemma
   (match apply_map_group_det m1 l with
   | MapGroupFail -> apply_map_group_det (m1 `map_group_concat` m2) l == MapGroupFail
-  | MapGroupDet l1 -> apply_map_group_det (m1 `map_group_concat` m2) l == apply_map_group_det m2 l1
+  | MapGroupDet c1 l1 ->
+    apply_map_group_det (m1 `map_group_concat` m2) l == begin match apply_map_group_det m2 l1 with
+    | MapGroupDet c2 l2 -> MapGroupDet (c1 `ghost_map_union` c2) l2
+    | res -> res
+    end
   | _ -> True)
   [SMTPat (apply_map_group_det (map_group_concat m1 m2) l)]
 
 val apply_map_group_det_mk_cut (cut: typ) (l: cbor_map) : Lemma
   (apply_map_group_det (map_group_mk_cut cut) l == (
     if List.Tot.for_all (notp (FStar.Ghost.Pull.pull (matches_map_group_entry cut any))) l
-    then MapGroupDet l
+    then MapGroupDet ghost_map_empty l
     else MapGroupFail
   ))
   [SMTPat (apply_map_group_det (map_group_mk_cut cut) l)]
@@ -244,7 +415,7 @@ val apply_map_group_det_match_item_for
   | None ->  MapGroupFail
   | Some x ->
     if ty x
-    then MapGroupDet (List.Tot.filter (notp (FStar.Ghost.Pull.pull (matches_map_group_entry (t_literal k) ty))) l)
+    then MapGroupDet (ghost_map_singleton k x) (List.Tot.filter (notp (FStar.Ghost.Pull.pull (matches_map_group_entry (t_literal k) ty))) l)
     else MapGroupFail
   ))
   [SMTPat (apply_map_group_det (map_group_match_item_for k ty) l)]
@@ -258,7 +429,7 @@ val apply_map_group_det_filter
   (l: cbor_map)
 : Lemma
   (apply_map_group_det (map_group_filter f) l ==
-    MapGroupDet (List.Tot.filter f l)
+    MapGroupDet (ghost_map_filter (notp f) (ghost_map_of_list l)) (List.Tot.filter f l)
   )
   [SMTPat (apply_map_group_det (map_group_filter f) l)]
 
@@ -273,14 +444,9 @@ let rec list_filter_filter (#t: Type) (p1 p2: t -> bool) (l: list t) : Lemma
   | [] -> ()
   | a :: q -> list_filter_filter p1 p2 q
 
-#restart-solver
-let map_group_filter_filter (p1 p2: (Cbor.raw_data_item & Cbor.raw_data_item) -> bool) : Lemma
+val map_group_filter_filter (p1 p2: (Cbor.raw_data_item & Cbor.raw_data_item) -> bool) : Lemma
   (map_group_filter p1 `map_group_concat` map_group_filter p2 == map_group_filter (andp p1 p2))
   [SMTPat (map_group_filter p1 `map_group_concat` map_group_filter p2)]
-= Classical.forall_intro (list_filter_filter p1 p2);
-  apply_map_group_det_map_group_equiv
-    (map_group_filter p1 `map_group_concat` map_group_filter p2)
-    (map_group_filter (andp p1 p2))
 
 let rec list_filter_ext (#t: Type) (p1 p2: t -> bool) (l: list t) : Lemma
   (requires forall (x: t) . List.Tot.memP x l ==> p1 x == p2 x)
@@ -294,6 +460,7 @@ let map_group_filter_ext (p1 p2: _ -> bool) : Lemma
   (requires forall x . p1 x == p2 x)
   (ensures map_group_filter p1 == map_group_filter p2)
 = Classical.forall_intro (Classical.move_requires (list_filter_ext p1 p2));
+  Classical.forall_intro (Classical.move_requires (ghost_map_filter_ext (notp p1) (notp p2)));
   apply_map_group_det_map_group_equiv
     (map_group_filter p1)
     (map_group_filter p2)
@@ -326,25 +493,11 @@ val map_group_zero_or_one_match_item_filter (key value: typ) (p: (Cbor.raw_data_
   )
   [SMTPat (map_group_zero_or_one (map_group_match_item key value) `map_group_concat` map_group_filter p)]
 
-val apply_map_group_det_zero_or_more_match_item
-  (key value: typ)
-  (l: cbor_map)
-: Lemma
-  (apply_map_group_det (map_group_zero_or_more (map_group_match_item key value)) l ==
-    MapGroupDet (List.Tot.filter (notp (FStar.Ghost.Pull.pull (matches_map_group_entry key value))) l)
-  )
-
-let map_zero_or_more_match_item_alt_eq
-  (key value: typ)
-: Lemma
+val map_group_zero_or_more_match_item_filter (key value: typ) : Lemma
   (map_group_zero_or_more (map_group_match_item key value) ==
     map_group_filter (notp (FStar.Ghost.Pull.pull (matches_map_group_entry key value)))
   )
   [SMTPat (map_group_zero_or_more (map_group_match_item key value))]
-= Classical.forall_intro (apply_map_group_det_zero_or_more_match_item key value);
-  apply_map_group_det_map_group_equiv
-    (map_group_zero_or_more (map_group_match_item key value))
-    (map_group_filter (notp (FStar.Ghost.Pull.pull (matches_map_group_entry key value))))
 
 let map_group_zero_or_more_match_item_choice_left
   (key1 key2 value: typ)
@@ -372,7 +525,7 @@ val matches_map_group (g: map_group) (m: cbor_map) : GTot bool
 val matches_map_group_det (g: map_group) (m: cbor_map) : Lemma
   (match apply_map_group_det g m with
   | MapGroupFail -> ~ (matches_map_group g m)
-  | MapGroupDet m' -> matches_map_group g m <==> m' == []
+  | MapGroupDet _ m' -> matches_map_group g m <==> m' == []
   | _ -> True)
 
 let t_map (g: map_group) : typ =
